Add calling compartment to call states.
For now, we leave out assembly language.

backend/CminorSel.v
@@ -143,6 +143,7 @@ Inductive state: Type :=
   | Callstate:                          (**r invocation of a fundef  *)
       forall (f: fundef)                (**r fundef to invoke *)
              (args: list val)           (**r arguments provided by caller *)
+             (cp: compartment)          (**r current compartment *)
              (k: cont)                  (**r what to do next  *)
              (m: mem),                  (**r memory state *)
       state
@@ -367,9 +368,9 @@ Inductive step: state -> trace -> state -> Prop :=
       Genv.find_funct ge vf = Some fd ->
       funsig fd = sig ->
       step (State f (Scall optid sig a bl) k sp e m)
-        E0 (Callstate fd vargs (Kcall optid f sp e k) m)
+        E0 (Callstate fd vargs f.(fn_comp) (Kcall optid f sp e k) m)
 
-  | step_tailcall: forall f sig a bl k sp e m vf vargs fd m',
+| step_tailcall: forall f sig a bl k sp e m vf vargs fd m',
       eval_expr_or_symbol (Vptr sp Ptrofs.zero) e m nil a vf ->
       eval_exprlist (Vptr sp Ptrofs.zero) e m nil bl vargs ->
       Genv.find_funct ge vf = Some fd ->
@@ -377,7 +378,7 @@ Inductive step: state -> trace -> state -> Prop :=
       forall COMP: comp_of fd = f.(fn_comp),
       Mem.free m sp 0 f.(fn_stackspace) = Some m' ->
       step (State f (Stailcall sig a bl) k (Vptr sp Ptrofs.zero) e m)
-        E0 (Callstate fd vargs (call_cont k) m')
+        E0 (Callstate fd vargs f.(fn_comp) (call_cont k) m')
 
   | step_builtin: forall f res ef al k sp e m vl t v m',
       list_forall2 (eval_builtin_arg sp e m) al vl ->
@@ -436,14 +437,14 @@ Inductive step: state -> trace -> state -> Prop :=
       step (State f (Sgoto lbl) k sp e m)
         E0 (State f s' k' sp e m)
 
-  | step_internal_function: forall f vargs k m m' sp e,
+  | step_internal_function: forall f vargs cp k m m' sp e,
       Mem.alloc m f.(fn_comp) 0 f.(fn_stackspace) = (m', sp) ->
       set_locals f.(fn_vars) (set_params vargs f.(fn_params)) = e ->
-      step (Callstate (Internal f) vargs k m)
+      step (Callstate (Internal f) vargs cp k m)
         E0 (State f f.(fn_body) k (Vptr sp Ptrofs.zero) e m')
-  | step_external_function: forall ef vargs k m t vres m',
+  | step_external_function: forall ef vargs cp k m t vres m',
       external_call ef ge vargs m t vres m' ->
-      step (Callstate (External ef) vargs k m)
+      step (Callstate (External ef) vargs cp k m)
          t (Returnstate vres k m')
 
   | step_return: forall v optid f sp e k m,
@@ -459,7 +460,7 @@ Inductive initial_state (p: program): state -> Prop :=
       Genv.find_symbol ge p.(prog_main) = Some b ->
       Genv.find_funct_ptr ge b = Some f ->
       funsig f = signature_main ->
-      initial_state p (Callstate f nil Kstop m0).
+      initial_state p (Callstate f nil default_compartment Kstop m0).
 
 Inductive final_state: state -> int -> Prop :=
   | final_state_intro: forall r m,
