backend/RTL.v
@@ -133,7 +133,7 @@ Fixpoint init_regs (vl: list val) (rl: list reg) {struct rl} : regset :=
   [pc] is the current program point (CFG node) within the code [c].
   [rs] gives the current values for the pseudo-registers.
   [m] is the current memory state.
-- [Callstate cs f args m] is an intermediate state that appears during
+- [Callstate cs f args cp m] is an intermediate state that appears during
   function calls.
   [f] is the function definition that we are calling.
   [args] (a list of values) are the arguments for this call.
@@ -174,6 +174,7 @@ Inductive state : Type :=
       forall (stack: list stackframe) (**r call stack *)
              (f: fundef)              (**r function to call *)
              (args: list val)         (**r arguments to the call *)
+             (cp: compartment)        (**r calling compartment *)
              (m: mem),                (**r memory state *)
       state
   | Returnstate:
@@ -234,7 +235,7 @@ Inductive step: state -> trace -> state -> Prop :=
       find_function ros rs = Some fd ->
       funsig fd = sig ->
       step (State s f sp pc rs m)
-        E0 (Callstate (Stackframe res f sp pc' rs :: s) fd rs##args m)
+        E0 (Callstate (Stackframe res f sp pc' rs :: s) fd rs##args f.(fn_comp) m)
   | exec_Itailcall:
       forall s f stk pc rs m sig ros args fd m',
       (fn_code f)!pc = Some(Itailcall sig ros args) ->
@@ -243,7 +244,7 @@ Inductive step: state -> trace -> state -> Prop :=
       forall COMP: comp_of fd = f.(fn_comp),
       Mem.free m stk 0 f.(fn_stacksize) = Some m' ->
       step (State s f (Vptr stk Ptrofs.zero) pc rs m)
-        E0 (Callstate s fd rs##args m')
+        E0 (Callstate s fd rs##args f.(fn_comp) m')
   | exec_Ibuiltin:
       forall s f sp pc rs m ef args res pc' vargs t vres m',
       (fn_code f)!pc = Some(Ibuiltin ef args res pc') ->
@@ -272,9 +273,9 @@ Inductive step: state -> trace -> state -> Prop :=
       step (State s f (Vptr stk Ptrofs.zero) pc rs m)
         E0 (Returnstate s (regmap_optget or Vundef rs) m')
   | exec_function_internal:
-      forall s f args m m' stk,
+      forall s f args cp m m' stk,
       Mem.alloc m f.(fn_comp) 0 f.(fn_stacksize) = (m', stk) ->
-      step (Callstate s (Internal f) args m)
+      step (Callstate s (Internal f) args cp m)
         E0 (State s
                   f
                   (Vptr stk Ptrofs.zero)
@@ -282,9 +283,9 @@ Inductive step: state -> trace -> state -> Prop :=
                   (init_regs args f.(fn_params))
                   m')
   | exec_function_external:
-      forall s ef args res t m m',
+      forall s ef args cp res t m m',
       external_call ef ge args m t res m' ->
-      step (Callstate s (External ef) args m)
+      step (Callstate s (External ef) args cp m)
          t (Returnstate s res m')
   | exec_return:
       forall res f sp pc rs s vres m,
@@ -328,7 +329,7 @@ Inductive initial_state (p: program): state -> Prop :=
       Genv.find_symbol ge p.(prog_main) = Some b ->
       Genv.find_funct_ptr ge b = Some f ->
       funsig f = signature_main ->
-      initial_state p (Callstate nil f nil m0).
+      initial_state p (Callstate nil f nil default_compartment m0).
 
 (** A final state is a [Returnstate] with an empty call stack. *)
 
