backend/Allocproof.v
@@ -1944,15 +1944,15 @@ Inductive match_states: RTL.state -> LTL.state -> Prop :=
       match_states (RTL.State s f sp pc rs m)
                    (LTL.State ts tf sp pc ls m')
   | match_states_call:
-      forall s f args m ts tf ls m'
+      forall s f args cp m ts tf ls m'
         (STACKS: match_stackframes s ts (funsig tf))
         (FUN: transf_fundef f = OK tf)
         (ARGS: Val.lessdef_list args (map (fun p => Locmap.getpair p ls) (loc_arguments (funsig tf))))
         (AG: agree_callee_save (parent_locset ts) ls)
         (MEM: Mem.extends m m')
         (WTARGS: Val.has_type_list args (sig_args (funsig tf))),
-      match_states (RTL.Callstate s f args m)
-                   (LTL.Callstate ts tf ls m')
+      match_states (RTL.Callstate s f args cp m)
+                   (LTL.Callstate ts tf ls cp m')
   | match_states_return:
       forall s res m ts ls m' sg
         (STACKS: match_stackframes s ts sg)
@@ -2322,6 +2322,7 @@ Proof.
   eapply star_right. eexact A1. econstructor; eauto.
   eauto. traceEq.
   exploit analyze_successors; eauto. simpl. left; eauto. intros [enext [U V]].
+  replace (fn_comp tf) with (RTL.fn_comp f) by apply (comp_transl_partial _ FUN).
   econstructor; eauto.
   econstructor; eauto.
   inv WTI. congruence.
@@ -2356,6 +2357,7 @@ Proof.
   replace (fn_stacksize tf) with (RTL.fn_stacksize f); eauto.
   destruct (transf_function_inv _ _ FUN); auto.
   eauto. traceEq.
+  replace (fn_comp tf) with (RTL.fn_comp f) by apply (comp_transl_partial _ FUN).
   econstructor; eauto.
   eapply match_stackframes_change_sig; eauto. rewrite SIG. rewrite e0. decEq.
   destruct (transf_function_inv _ _ FUN); auto.
@@ -2505,7 +2507,7 @@ Proof.
   intros. inv H.
   exploit function_ptr_translated; eauto. intros [tf [FIND TR]].
   exploit sig_function_translated; eauto. intros SIG.
-  exists (LTL.Callstate nil tf (Locmap.init Vundef) m0); split.
+  exists (LTL.Callstate nil tf (Locmap.init Vundef) default_compartment m0); split.
   econstructor; eauto.
   eapply (Genv.init_mem_transf_partial TRANSF); eauto.
   rewrite symbols_preserved.
