backend/Constpropproof.v
@@ -304,13 +304,13 @@ Inductive match_states: nat -> state -> state -> Prop :=
       match_states n (State s f sp pc rs m)
                     (State s' (transf_function (romem_for cu) f) sp pc' rs' m')
   | match_states_call:
-      forall s f args m s' args' m' cu
+      forall s f args cp m s' args' m' cu
            (LINK: linkorder cu prog)
            (STACKS: list_forall2 match_stackframes s s')
            (ARGS: Val.lessdef_list args args')
            (MEM: Mem.extends m m'),
-      match_states O (Callstate s f args m)
-                     (Callstate s' (transf_fundef (romem_for cu) f) args' m')
+      match_states O (Callstate s f args cp m)
+                     (Callstate s' (transf_fundef (romem_for cu) f) args' cp m')
   | match_states_return:
       forall s v m s' v' m'
            (STACKS: list_forall2 match_stackframes s s')
@@ -588,7 +588,7 @@ Lemma transf_initial_states:
 Proof.
   intros. inversion H.
   exploit function_ptr_translated; eauto. intros (cu & FIND & LINK).
-  exists O; exists (Callstate nil (transf_fundef (romem_for cu) f) nil m0); split.
+  exists O; exists (Callstate nil (transf_fundef (romem_for cu) f) nil default_compartment m0); split.
   econstructor; eauto.
   apply (Genv.init_mem_match TRANSL); auto.
   replace (prog_main tprog) with (prog_main prog).
