backend/Deadcodeproof.v
@@ -517,14 +517,14 @@ Inductive match_states: state -> state -> Prop :=
       match_states (State s f (Vptr sp Ptrofs.zero) pc e m)
                    (State ts tf (Vptr sp Ptrofs.zero) pc te tm)
   | match_call_states:
-      forall s f args m ts tf targs tm cu
+      forall s f args cp m ts tf targs tm cu
         (STACKS: list_forall2 match_stackframes s ts)
         (LINK: linkorder cu prog)
         (FUN: transf_fundef (romem_for cu) f = OK tf)
         (ARGS: Val.lessdef_list args targs)
         (MEM: Mem.extends m tm),
-      match_states (Callstate s f args m)
-                   (Callstate ts tf targs tm)
+      match_states (Callstate s f args cp m)
+                   (Callstate ts tf targs cp tm)
   | match_return_states:
       forall s v m ts tv tm
         (STACKS: list_forall2 match_stackframes s ts)
@@ -875,6 +875,7 @@ Ltac UseTransfer :=
   exploit find_function_translated; eauto 2 with na. intros (cu' & tfd & A & B & C).
   econstructor; split.
   eapply exec_Icall; eauto. eapply sig_function_translated; eauto.
+  rewrite comp_transf_function; eauto.
   eapply match_call_states with (cu := cu'); eauto.
   constructor; auto. eapply match_stackframes_intro with (cu := cu); eauto.
   intros.
@@ -894,6 +895,7 @@ Ltac UseTransfer :=
   eapply exec_Itailcall; eauto. eapply sig_function_translated; eauto.
   rewrite <- (comp_transl_partial _ B), COMP. now apply (comp_transl_partial _ FUN).
   erewrite stacksize_translated by eauto. eexact C.
+  rewrite comp_transf_function; eauto.
   eapply match_call_states with (cu := cu'); eauto 2 with na.
   eapply magree_extends; eauto. apply nlive_all.
 
@@ -1125,7 +1127,7 @@ Lemma transf_initial_states:
 Proof.
   intros. inversion H.
   exploit function_ptr_translated; eauto. intros (cu & tf & A & B & C).
-  exists (Callstate nil tf nil m0); split.
+  exists (Callstate nil tf nil default_compartment m0); split.
   econstructor; eauto.
   eapply (Genv.init_mem_match TRANSF); eauto.
   replace (prog_main tprog) with (prog_main prog).
