backend/Linearizeproof.v
@@ -547,11 +547,11 @@ Inductive match_states: LTL.state -> Linear.state -> Prop :=
       match_states (LTL.Block s f sp bb ls m)
                    (Linear.State ts tf sp (linearize_block bb c) ls m)
   | match_states_call:
-      forall s f ls m tf ts,
+      forall s f ls cp m tf ts,
       list_forall2 match_stackframes s ts ->
       transf_fundef f = OK tf ->
-      match_states (LTL.Callstate s f ls m)
-                   (Linear.Callstate ts tf ls m)
+      match_states (LTL.Callstate s f ls cp m)
+                   (Linear.Callstate ts tf ls cp m)
   | match_states_return:
       forall s ls m ts,
       list_forall2 match_stackframes s ts ->
@@ -639,6 +639,7 @@ Proof.
   left; econstructor; split. simpl.
   apply plus_one. econstructor; eauto.
   symmetry; eapply sig_preserved; eauto.
+  replace (LTL.fn_comp f) with (fn_comp tf) by (symmetry; apply (comp_transl_partial _ TRF)).
   econstructor; eauto. constructor; auto. econstructor; eauto.
 
   (* Ltailcall *)
@@ -650,6 +651,7 @@ Proof.
   now rewrite <- (comp_transl_partial _ B), <- (comp_transl_partial _ TRF).
   rewrite (stacksize_preserved _ _ TRF); eauto.
   rewrite (match_parent_locset _ _ STACKS).
+  replace (LTL.fn_comp f) with (fn_comp tf) by (symmetry; apply (comp_transl_partial _ TRF)).
   econstructor; eauto.
 
   (* Lbuiltin *)
@@ -703,7 +705,7 @@ Proof.
   (* internal functions *)
   assert (REACH: (reachable f)!!(LTL.fn_entrypoint f) = true).
     apply reachable_entrypoint.
-  monadInv H7.
+  monadInv H8.
   left; econstructor; split.
   apply plus_one. eapply exec_function_internal; eauto.
   rewrite (stacksize_preserved _ _ EQ).
@@ -712,7 +714,7 @@ Proof.
   econstructor; eauto. simpl. eapply is_tail_add_branch. constructor.
 
   (* external function *)
-  monadInv H8. left; econstructor; split.
+  monadInv H9. left; econstructor; split.
   apply plus_one. eapply exec_function_external; eauto.
   eapply external_call_symbols_preserved; eauto. apply senv_preserved.
   econstructor; eauto.
@@ -730,7 +732,7 @@ Lemma transf_initial_states:
 Proof.
   intros. inversion H.
   exploit function_ptr_translated; eauto. intros [tf [A B]].
-  exists (Callstate nil tf (Locmap.init Vundef) m0); split.
+  exists (Callstate nil tf (Locmap.init Vundef) default_compartment m0); split.
   econstructor; eauto. eapply (Genv.init_mem_transf_partial TRANSF); eauto.
   rewrite (match_program_main TRANSF).
   rewrite symbols_preserved. eauto.
