backend/Stackingproof.v
@@ -1791,7 +1791,7 @@ Inductive match_states: Linear.state -> Mach.state -> Prop :=
       match_states (Linear.State cs f (Vptr sp Ptrofs.zero) c ls m)
                    (Mach.State cs' fb (Vptr sp' Ptrofs.zero) (transl_code (make_env (function_bounds f)) c) rs m')
   | match_states_call:
-      forall cs f ls m cs' fb rs m' j tf
+      forall cs f ls cp m cs' fb rs m' j tf
         (STACKS: match_stacks j cs cs' (Linear.funsig f))
         (TRANSL: transf_fundef f = OK tf)
         (FIND: Genv.find_funct_ptr tge fb = Some (tf))
@@ -1799,8 +1799,8 @@ Inductive match_states: Linear.state -> Mach.state -> Prop :=
         (SEP: m' |= stack_contents j cs cs'
                  ** minjection j m
                  ** globalenv_inject ge j),
-      match_states (Linear.Callstate cs f ls m)
-                   (Mach.Callstate cs' fb rs m')
+      match_states (Linear.Callstate cs f ls cp m)
+                   (Mach.Callstate cs' fb rs cp m')
   | match_states_return:
       forall cs ls m cs' rs m' j sg
         (STACKS: match_stacks j cs cs' sg)
@@ -1958,6 +1958,7 @@ Proof.
   exploit return_address_offset_exists. eexact IST. intros [ra D].
   econstructor; split.
   apply plus_one. econstructor; eauto.
+  replace (fn_comp tf) with (Linear.fn_comp f) by apply (comp_transf_function _ _ TRANSL).
   econstructor; eauto.
   econstructor; eauto with coqlib.
   apply Val.Vptr_has_type.
@@ -1976,6 +1977,7 @@ Proof.
   intros [bf [tf' [A [B C]]]].
   econstructor; split.
   eapply plus_right. eexact S. econstructor; eauto. traceEq.
+  replace (fn_comp tf) with (Linear.fn_comp f) by apply (comp_transf_function _ _ TRANSL).
   econstructor; eauto.
   apply match_stacks_change_sig with (Linear.fn_sig f); auto.
   apply zero_size_arguments_tailcall_possible. eapply wt_state_tailcall; eauto.
