cfrontend/SimplLocalsproof.v
@@ -1770,15 +1770,15 @@ Inductive match_states: state -> state -> Prop :=
       match_states (State f s k e le m)
                    (State tf ts tk te tle tm)
   | match_call_state:
-      forall fd vargs k m tfd tvargs tk tm j targs tres cconv
+      forall fd vargs cp k m tfd tvargs tk tm j targs tres cconv
         (TRFD: transf_fundef fd = OK tfd)
         (MCONT: forall cenv, match_cont j cenv k tk m (Mem.nextblock m) (Mem.nextblock tm))
         (MINJ: Mem.inject j m tm)
         (AINJ: Val.inject_list j vargs tvargs)
         (FUNTY: type_of_fundef fd = Tfunction targs tres cconv)
         (ANORM: val_casted_list vargs targs),
-      match_states (Callstate fd vargs k m)
-                   (Callstate tfd tvargs tk tm)
+      match_states (Callstate fd vargs cp k m)
+                   (Callstate tfd tvargs cp tk tm)
   | match_return_state:
       forall v k m tv tk tm j
         (MCONT: forall cenv, match_cont j cenv k tk m (Mem.nextblock m) (Mem.nextblock tm))
@@ -2068,6 +2068,7 @@ Proof.
   rewrite typeof_simpl_expr. eauto.
   eauto. eauto. eauto.
   erewrite type_of_fundef_preserved; eauto.
+  replace (fn_comp tf) with (fn_comp f) by now apply comp_transl_partial.
   econstructor; eauto.
   intros. econstructor; eauto.
 
